compiler/src/compiler/FlatToRiscvSimulation.v
@@ -47,16 +47,19 @@ Section Sim.
     fun '(e, c, done, t, m, l) st =>
         e = g.(e_impl) /\
         fits_stack g.(num_stackwords) g.(e_impl) c /\
-        (forall f argnames retnames body,
+        (* TODO factor out this forall *)
+        (forall f (argnames retnames: list Syntax.varname) (body: stmt),
             map.get g.(e_impl) f = Some (argnames, retnames, body) ->
-            Forall valid_register argnames /\
-            Forall valid_register retnames /\
-            valid_registers body /\
+            Forall valid_FlatImp_var argnames /\
+            Forall valid_FlatImp_var retnames /\
+            valid_FlatImp_vars body /\
+            NoDup argnames /\
+            NoDup retnames /\
             stmt_not_too_big body /\
             In f g.(funnames) /\
             (exists pos : Z, map.get g.(e_pos) f = Some pos /\ pos mod 4 = 0)) /\
         stmt_not_too_big c /\
-        valid_registers c /\
+        valid_FlatImp_vars c /\
         compile_stmt_new g.(e_pos) pos c = g.(insts) /\
         pos mod 4 = 0 /\
         regs_initialized st.(getRegs) /\
